tests/defined/malloc_nondet.c
@@ -1,0 +1,7 @@
+int main() {
+  if(malloc(1)) {
+    printf("foo\n");
+  } else {
+    printf("bar\n");
+  }
+}
