architectures.v
@@ -2,7 +2,7 @@
 (* This file is distributed under the terms of the BSD license. *)
 Require Export architecture_spec.
 
-Definition x86 : architecture.
+Definition x86 (alloc_can_fail : bool) : architecture.
 Proof.
  refine {|
   arch_big_endian := false;
@@ -18,11 +18,12 @@ Proof.
     | CharRank => 1 | ShortRank => 2 | IntRank | LongRank => 4
     | LongLongRank => 4
     end;
-  arch_ptr_rank := LongRank
+  arch_ptr_rank := LongRank;
+  arch_alloc_can_fail := alloc_can_fail
  |}; by apply (bool_decide_unpack _); vm_compute.
 Defined.
 
-Definition x86_64 : architecture.
+Definition x86_64 (alloc_can_fail : bool) : architecture.
 Proof.
  refine {|
   arch_big_endian := false;
@@ -38,6 +39,7 @@ Proof.
     | CharRank => 1 | ShortRank => 2 | IntRank => 4
     | LongRank | LongLongRank => 8
     end;
-  arch_ptr_rank := LongRank
+  arch_ptr_rank := LongRank;
+  arch_alloc_can_fail := alloc_can_fail
  |}; by apply (bool_decide_unpack _); vm_compute.
 Defined.
